\documentclass{article}
\usepackage{amsthm}

\newtheorem*{Theorem}{Generalized Gauss-Markov Theorem}
\newtheorem*{Assumption}{Assumption}
\begin{document}
\begin{Theorem}
  \begin{Assumption}
  	~\\
  	Y=X$\beta$+e\\
  	$where$ E$\lbrack$e$\mid$X$\rbrack$=0 \quad 
  	var$\lbrack$e$\mid$X$\rbrack$=$\Omega$\quad
  	E$\lbrack$$Y^2$$\mid$X$\rbrack$ \textless$\infty$\quad
  	E$\lbrack$$X^{2}$$\rbrack$$<$$\infty$\\
  	$X^{T}X$ $is$ $invertible$
  \end{Assumption}
  ~\\
  Under the given assumption and $\Omega$$>$0, let $\tilde{\beta}$ be a linear unbiased estimator of $\beta$ then we have\\ 
  \begin{center}$ var\lbrack\tilde{\beta}\mid X\rbrack\geq(X^{T}\Omega^{-1}X)^{-1}$\end{center}
\end{Theorem}
\linespread{1.5}
\begin{proof}
	~\\
	let $\tilde{\beta}$=CY where C is a function of X. \\
	E[$\tilde{\beta}$$\mid$X]=E[CY$\mid$X]\\
	=E[C(X$\beta$+e)$\mid$X]\\
	=E[CX$\beta$+Ce$\mid$X]\\
	=CX$\beta$\\
	=$\beta$\\
	Thus CX=I\\
	var[$\tilde{\beta}$$\mid$X]=var[$(Ce)$$\mid$X]=$C$var[e$\mid$X]$C^{T}$=$C$$\Omega$$C^{T}$\\
	Without loss of generality, let $C$=$(X^{T}\Omega^{-1}X)^{-1}X^{T}\Omega^{-1}+D$\\
	CX=I $\Rightarrow$ DX=0\\
	Note that $\Omega$ is positive semi-definite and symmetry,\\
	Thus,\\ var[$\tilde{\beta}$$\mid$X]=$C$$\Omega$$C^{T}$\\
	=$((X^{T}\Omega^{-1}X)^{-1}X^{T}\Omega^{-1}+D)\Omega(D^{T}+(\Omega^{-1})^{T}X(X^{T}\Omega^{-1}X)^{-1})$\\
	=$(X^{T}\Omega^{-1}X)^{-1}X^{T}\Omega^{-1}X(X^{T}\Omega^{-1}X)^{-1}+D \Omega D^{T}$\\
	=$(X^{T}\Omega^{-1}X)^{-1}+D \Omega D^{T}$
	$\geq$$(X^{T}\Omega^{-1}X)^{-1}$
\end{proof}
\end{document}